update Zulib

src/Zulib/fstar/Zen.IList.fst
@@ -19,18 +19,17 @@ type ilist (a:Type) = l:list (a ** nat){ is_ilist l}
 // for qualified import
 type t (a:Type) = ilist a
 
-val ilist_tl(#a:Type): l:ilist a ->
+val ilist_tl_ilist(#a:Type): l:ilist a ->
     Lemma ( match l with
             | [] -> True
             | hd::tl -> is_ilist tl )
-let ilist_tl #_ _ = ()
+let ilist_tl_ilist #_ _ = ()
 
 (* gets the length of an ilist *)
 val length(#a:Type): ilist a -> nat
 let length(#a:Type) = function
     | [] -> 0
     | (_,n)::_ -> n
-
 
 val length_tl(#a:Type):
     l:ilist a{Cons? l}
@@ -44,12 +43,66 @@ let cons #_ x l =
     | [] -> 2 +~! [x,1]
     | (_,n)::_ -> 2 +~! (x, n+1)::l
 
+val (::) (#a:Type): a -> ilist a -> ilist a `cost` 2
+let (::) #_ x l = cons x l
+
 val cons_length(#a:Type):
     x:a
     -> ls:ilist a
     -> Lemma ( let result = force (cons x ls) in
                length result == length ls + 1 )
 let cons_length #_ _ _ = ()
+
+val head(#a:Type): ls:ilist a{length ls >= 1} -> a `cost` 1
+let head #_ ((hd,_)::_) = 1 +~! hd
+
+val tryHead(#a:Type): ls:ilist a -> option a `cost` 2
+let tryHead #_ = function
+    | [] -> 2 +~! None
+    | (hd,_)::_ -> 2 +~! Some hd
+
+val tail(#a:Type): ls:ilist a{length ls >= 1} -> ilist a `cost` 1
+let tail #_ (_::tl) = 1 +~! tl
+
+val tryTail(#a:Type): ls:ilist a -> option (ilist a) `cost` 2
+let tryTail #_ = function
+    | [] -> 2 +~! None
+    | _::tl -> 2 +~! Some tl
+
+val nth(#a:Type): ls:ilist a -> n:nat{n < length ls} -> a `cost` (4 * n + 4)
+let rec nth #_ ls n = match ls with
+    | (hd,_)::tl -> if n = 0 then 4 +~! hd else 4 +! nth tl (n-1)
+
+val tryNth(#a:Type): ilist a -> n:nat -> option a `cost` (4 * n + 4)
+let rec tryNth #_ ls n = match ls with
+    | [] -> (4*n+4) +~! None
+    | (hd,_)::tl -> if n = 0 then 4 +~! Some hd else 4 +! tryNth tl (n-1)
+
+val append(#a:Type): l1:ilist a -> l2:ilist a -> ilist a `cost` (4 * length l1 + 4)
+let rec append #a l1 l2 = match l1 with
+    | [] -> 4 +~! l2
+    | (l1_hd,_)::l1_tl ->
+        let l1_tl : ilist a = l1_tl in
+        let! tl = append l1_tl l2 in
+        2 +! cons l1_hd tl
+
+val (++) (#a:Type): l1:ilist a -> l2:ilist a -> ilist a `cost` (4 * length l1 + 4)
+let (++) #_ l1 l2 = append l1 l2
+
+val rev_append(#a:Type): l1:ilist a -> l2:ilist a -> ilist a `cost` (4 * length l1 + 4)
+let rec rev_append #a l1 l2 = match l1 with
+    | [] -> 4 +~! l2
+    | (hd,_)::tl ->
+        let tl : ilist a = tl in
+        let! l2 = 2 +! (cons hd l2) in
+        rev_append tl l2
+
+val rev (#a:Type): ls:ilist a -> ilist a `cost` (4 * length ls + 4)
+let rev #_ ls = rev_append ls []
+
+// TODO : init
+// TODO : flatten
+// TODO : concat
 
 val map(#a #b:Type):
     (a -> b)
@@ -81,7 +134,7 @@ let rec mapT #a #_ #_ f = function
         let tl: ilist a = tl in
         let tl = f `mapT` tl in
         1 +! (bind2 (f hd) tl cons)
-
+(*
 val mapT_cons(#a #b:Type)(#n:nat):
     f:(a -> b `cost` n)
     -> ls:ilist a
@@ -106,7 +159,7 @@ let rec mapT_length #a #_ #_ f ls =
         let tl: ilist a = tl in
         mapT_length f tl;
         mapT_cons f ls
-
+*)
 val foldl(#a #b:Type):
     (a -> b -> a)
     -> a
@@ -146,46 +199,3 @@ val sumByT(#a:Type)(#n:nat):
     -> int `cost` ((3 + n) * length ls + 3 )
 let sumByT #_ #n f =
     foldlT (fun acc x -> (+) acc `Cost.map` f x) 0
-(*)
-type ilist' (a:Type) =
-    | INil : ilist' a
-    | ICons : hd:a -> tl:ilist' a -> n:nat -> ilist' a
-
-private val is_ilist(#a:Type): ilist' a -> Type0
-private let rec is_ilist #_ = function
-    | INil -> True
-    | ICons hd tl n ->
-        is_ilist tl /\
-        begin match tl with
-        | INil -> n == 1
-        | ICons _ _ n' -> n == n' + 1
-        end
-
-type ilist (a:Type) = l:ilist' a{is_ilist l}
-
-
-val tl_ilist(#a:Type): l:ilist a
-    -> Lemma ( match l with
-               | INil -> True
-               | ICons _ tl _ -> is_ilist tl )
-let tl_ilist #_ _ = ()
-
-val iCons(#a:Type): a -> ilist a -> ilist a
-let iCons #_ x l =
-    match l with
-    | INil -> ICons x INil 1
-    | ICons _ _ n -> ICons x l (n+1)
-
-val ilength(#a:Type): ilist a -> nat
-let ilength(#a:Type) = function
-    | INil -> 0
-    | ICons _ _ n -> n
-
-val imap(#a #b:Type): (a -> b) -> l:ilist a -> ilist b `cost` ilength l
-let rec imap #a #_ f l =
-    match l with
-    | INil -> ret INil
-    | ICons hd tl n ->
-        let tl = tl <: ilist a in
-        let! ftl = f `imap` tl in
-        1 +~! iCons (f hd) ftl n
