src/Zulib/fstar/Zen.Dictionary.fsti
@@ -5,15 +5,104 @@ open Zen.Cost
 (* A dictionary is a map from `string` to some other type. *)
 assume new type dictionary (t:Type u#a) : Type u#a
 assume Dictionary_hasEq: forall (a:eqtype). hasEq (dictionary a)
-
+// for qualified imports
 type t (a:Type) = dictionary a
 
+(* Returns the number of elements in the dictionary *)
+val size(#a:Type): dictionary a -> nat
+
+(* Returns `true` if the dictionary contains the given key. *)
+val containsKey(#a:Type): key:string -> dictionary a -> bool `cost` 64
+// if a dictionary contains a key k, then it's size is at least 1,
+// and if a dictionary has a size of at least 1, then it must contain a key.
+assume ContainsSize: forall (a:Type) (d:dictionary a).
+    (exists (k:string). force (containsKey k d) = true) <==> size d >= 1
+
+(* Returns the value with key `k`, if it exists. *)
+val tryFind(#a:Type): k:string -> dictionary a -> option a `cost` 64
+assume TryFindContainsKey: forall (a:Type) (d:dictionary a) (k:string).
+    let result = force (tryFind k d) in
+    let d_contains_k = force (containsKey k d) in
+    (d_contains_k = true <==> Some? result)
+    /\
+    (d_contains_k = false <==> None? result)
+
+(* Adds `value` to a dictionary with key `k`. *)
+val add(#a:Type): k:string -> value:a -> dictionary a -> dictionary a `cost` 64
+// adding a value v with key k to a dictionary:
+//     increases it's size by 1 if it does not contain the key
+//     does not change it's size if it does contain the key
+assume AddSize: forall (a:Type) (d:dictionary a) (k:string) (v:a).
+    let result = force (add k v d) in
+    let d_contains_k = force (containsKey k d) in
+    (d_contains_k = true <==> size result == size d)
+    /\
+    (d_contains_k = false <==> size result == size d + 1)
+// if a key exists in a dictionary, then it also exists after an add.
+assume AddKey: forall (a:Type) (d:dictionary a) (k:string) (v:a).
+    let result = force (add k v d) in
+    let d_contains_k = force (containsKey k d) in
+    let result_contains_k = force (containsKey k result) in
+    d_contains_k = true ==> result_contains_k = true
+// if a dictionary does not contain the key k2, then for a key k1 =/= k2,
+// k2 does not exist after adding k1.
+assume AddKeyNegative: forall (a:Type) (d:dictionary a) (k1 k2:string) (v:a).
+    let result = force (add k1 v d) in
+    let d_contains_k2 = force (containsKey k2 d) in
+    let result_contains_k2 = force (containsKey k2 result) in
+    ((k1 <> k2) /\ d_contains_k2 = false) <==> result_contains_k2 = false
+// the value at k1 after adding v add at k1 is v.
+// the value of k2 after adding v at k1 is the value of k2 in d, if k1 =/= k2.
+assume AddTryFind: forall (a:Type) (d:dictionary a) (k1 k2:string) (v:a).
+    let result = force (add k1 v d) in
+    let d_k2 = force (tryFind k2 d) in
+    let result_k1 = force (tryFind k1 result) in
+    let result_k2 = force (tryFind k2 result) in
+    (result_k1 == Some v)
+    /\
+    ((k1 <> k2) ==> result_k2 == d_k2)
+
+(* Removes a key-value pair from a dictionary,
+   if the key `k` exists in the dictionary. *)
+val remove(#a:Type): k:string -> dictionary a -> dictionary a `cost` 64
+// removing a key from a dictionary:
+//     decreases it's size by 1 if it contains the key
+//     does not change it's size if it does not contain the key
+assume RemoveSize: forall (a:Type) (d:dictionary a) (k:string).
+    let result = force (remove k d) in
+    let d_contains_k = force (containsKey k d) in
+    (d_contains_k = true <==> size result == size d - 1)
+    /\
+    (d_contains_k = false <==> size result == size d)
+// if a key exists in a dictionary, then it does not exist after a removal.
+assume RemoveKey: forall (a:Type) (d:dictionary a) (k:string).
+    let result = force (remove k d) in
+    force (containsKey k result) = false
+// if a dictionary contains a key k2, and k2 =/= k1,
+// then k2 exists after a removal of k1.
+assume RemoveKeyNegative: forall (a:Type) (d:dictionary a) (k1 k2:string).
+    let result = force (remove k1 d) in
+    let d_contains_k2 = force (containsKey k2 d) in
+    let result_contains_k2 = force (containsKey k2 result) in
+    ((k1 <> k2) /\ d_contains_k2 = true) <==> result_contains_k2 = true
+// the value at k1 after removing k1 is None.
+// the value of k2 after removing k1 is the value of k2 in d, if k1 =/= k2.
+assume AddTryFind: forall (a:Type) (d:dictionary a) (k1 k2:string).
+    let result = force (remove k1 d) in
+    let d_k2 = force (tryFind k2 d) in
+    let result_k1 = force (tryFind k1 result) in
+    let result_k2 = force (tryFind k2 result) in
+    (result_k1 == None)
+    /\
+    ((k1 <> k2) ==> result_k2 == d_k2)
+
+(* an empty dictionary *)
 val empty(#a:Type): dictionary a
-
-val add(#a:Type): string -> a -> dictionary a -> dictionary a `cost` 64
-
-val containsKey(#a:Type): string -> dictionary a -> bool `cost` 64
-
-val remove(#a:Type): string -> dictionary a -> dictionary a `cost` 64
-
-val tryFind(#a:Type): string -> dictionary a -> option a `cost` 64
+// Empty dictionary has 0 size
+assume EmptySize: forall (a:Type). size (empty #a) == 0
+// Empty dictionary is the only dictionary with size 0
+assume EmptyUnique: forall (a:Type) (d:dictionary a).
+    size d = 0 <==> d == empty
+// Empty dictionary does not contain any key.
+assume EmptyContainsKey: forall (a:Type) (key:string).
+    force (containsKey key (empty #a)) == false
